\documentclass{unswmaths}

\usepackage{unswshortcuts}

\begin{document}

\subject{Galois Theory}
\author{Edward McDonald}
\title{Assignment 1}
\studentno{3375335}


\setlength\parindent{0pt}


\unswtitle{}

    For this assignment, $n > 1$ and $k$ is a field
    containing a primitive $n$th root of unity $\zeta_n$,
    and the characteristic of $k$ does not divide $n$.
    
    Let $a \in k$ be such that the polynomial
    $P_a(x) = x^n-a$ has no root in $k$.
    
    Let $K_{a,n} = k(\!\sqrt[n]{a})$ be a field extention
    of $k$ generated by a root of $P_a$.

\section*{Question 1}
\begin{lemma}
    In $K_{a,n}$, $P_a$ is expressed as a product of $n$ distinct linear
    factors 
    \begin{equation*}
        P_a(x) = \prod_{k=1}^n (x-\zeta_n^k\sqrt[n]{a})
    \end{equation*}
\end{lemma}
\begin{proof}
    Since $\zeta_n$ is primitive, all
    of the elements $\zeta_n^k\sqrt[n]{a}$ for $k = 1,2,\ldots,n$
    are distinct and are all zeroes of $P_a$.
    
    Hence since $P_a$ has at most $n$ roots, this is all of the roots
    of $P_a$ and so $P_a$ decomposes as
    \begin{equation*}
        P_a(x) = \prod_{k=1}^n (x-\zeta_n^k\sqrt[n]{a})
    \end{equation*}
\end{proof}

\section*{Question 2}
For this question, $\lambda \in \Intgr/n\Intgr$ and 
define
\begin{equation*}
    \sigma_\lambda: K_{a,n}\rightarrow K_{a,n}
\end{equation*}
by $\sigma_{\lambda}(f(\sqrt[n]{a})) = f(\zeta_n^\lambda \sqrt[n]{a})$
for any polynomial $f \in k[x]$.
\begin{theorem}
    $\sigma_\lambda$ is a field automorphism on $K_{a,n}$.
\end{theorem}
\begin{proof}
    First since any $x \in K_{a,n}$
    can be written uniquely as a sum
    \begin{equation*}
        x = b_0 + b_1\sqrt[n]{a}+b_2\sqrt[n]{a^2} + \cdots + b_{n-1}\sqrt[n]{a^{n-1}},
    \end{equation*}
    for $b_i \in k$, then $\sigma_\lambda(x)$ is given by
    \begin{equation*}
        \sigma_\lambda(x) = b_0 + b_1\sqrt[n]{a}\zeta_n^\lambda+b_2\sqrt[n]{a^2}\zeta_n^{2\lambda}+\cdots+b_{n-1}\sqrt[n]{a^{n-1}}\zeta_n^{\lambda(n-1)}.
    \end{equation*}
    
    Suppose that $f(\sqrt[n]{a}),g(\sqrt[n]{a}) \in K_{a,n}$. Then,
    \begin{align*}
        \sigma_{\lambda}(f(\sqrt[n]{a})+g(\sqrt[n]{a}) &= \sigma_\lambda((f+g)(\sqrt[n]{a}))\\
        &= (f+g)(\sqrt[n]{a}\zeta_n^\lambda)\\
        &= f(\sqrt[n]{a}\zeta_n^\lambda) + g(\sqrt[n]{a}\zeta_n^\lambda)\\
        &= \sigma_\lambda(f(\sqrt[n]{a}))+\sigma_\lambda(g(\sqrt[n]{a})).
    \end{align*}
    Hence the function $\sigma_\lambda$ is additive. An identical argument shows that $\sigma_\lambda$
    is multiplicative.
    
    Since for $b \in k$, $\sigma_\lambda(bf(\sqrt[n]{a})) = b\sigma_\lambda(f(\sqrt[n]{a}))$,
    
\end{proof}

\section*{Question 3}
\begin{lemma}
    If $\sigma \in \Aut(K_{a,n}/k)$, then $P_a(\sigma(\sqrt[n]{a})) = 0$.
\end{lemma}
\begin{proof}
    We simply compute $P_a(\sigma(\sqrt[n]{a}))$,
    \begin{align*}
        P(\sigma(\sqrt[n]{a})) &= \sigma(\sqrt[n]{a})^n-a\\
        &= \sigma(\sqrt[n]{a}^n)-a\\
        &= \sigma(a)-\sigma(a)\\
        &= 0.
    \end{align*}
\end{proof}
\begin{lemma}
    If $\sigma \in \Aut(K_{a,n}/k)$, then $\sigma = \sigma_\lambda$ for some $\lambda \in \Intgr/n$. 
\end{lemma}
\begin{proof}
    We have shown that $\sigma(\sqrt[n]{a})$ is a root of $P_a$, however the only roots of $P_{a}$ over
    $K_{a,n}$ are of the form $\zeta_{n}^\lambda \sqrt[n]{a}$ for some $\lambda \in \Intgr/n$. 
    Hence $\sigma(\sqrt[n]{a}) = \zeta_n^\lambda \sqrt[n]{a}$. Since $\{1,\sqrt[n]{a}\}$
    generates $K_{a,n}$ as a $k$-space, this uniquely determines $\sigma$ as $\sigma_\lambda$.
\end{proof}
\begin{theorem}
    Hence, $\Aut(K_{a,n}/k)$ is isomorphic to $\Intgr/n$ as a group.
\end{theorem}
\begin{proof}
    The map $\lambda \mapsto \sigma_\lambda$ is a bijection since we
    have shown that it is surjective, and if $\sigma_\lambda = \sigma_\mu$, then
    $\zeta_n^\lambda = \zeta_n^\mu$ so $\lambda = \mu$ as $\zeta_n$ is primitive.
    
    To show that this is a group homomorphism, let $\lambda,\mu \in \Intgr/n$.
    Then $\sigma_\lambda\circ\sigma_\mu$ is a field automorphism fixing $k$,
    and $\sigma_\lambda(\sigma_\mu(\sqrt[n]{a})) = \sqrt[n]{a}\zeta_n^\mu\zeta_n^\lambda = \sqrt[n]{a}\zeta_n^{\lambda+\mu}$.
    
    Hence $\sigma_\lambda\circ \sigma_\mu = \sigma_{\lambda+\mu}$.
    
    Hence we have an isomorphism of groups.
\end{proof} 
    
\section*{Question 4}
For this question, $m|n$ is an integer, and $m(\Intgr/n)$ is the subgroup of $\Intgr/n$
generated by $m$.
\begin{lemma}
    $\sqrt[m]{a}$ is fixed by $\sigma_\lambda$ for each $\lambda \in m(\Intgr/n)$.
\end{lemma}
\begin{proof}
    Note that $\sqrt[m]{a} = \sqrt[n]{a}^{n/m}$ since $n/m$ is an integer. 
    Hence $\sigma_\lambda(\sqrt[m]{a}) = \sqrt[n]{a}^{n/m}\zeta_n^{n\lambda/m} = \sqrt[n]{a}\zeta_n^{n\lambda/m}$
    Hence $\sigma_\lambda$ fixed $\sqrt[n]{a}$ if and only if $n| n\lambda/m$, so we must have $m|\lambda$.
    Hence $\lambda \in m(\Intgr/n)$.
\end{proof}

\begin{theorem}
    $\sigma_\lambda(u) = u$ for all $\lambda \in m(\Intgr/n)$ if and only if $u \in K_{a,m}$.
\end{theorem}
\begin{proof}
    Suppose first that $u \in K_{a,m}$. It is sufficient to prove that case $u = \sqrt[m]{a}$
    since $\sqrt[m]{a}$ generates $K_{a,m}$. We have already shown for this case that $\sigma_\lambda(u) = u$
    for all $\lambda \in m(\Intgr/n)$.
    
    Conversely, assume that $\sigma_\lambda(u) = u$ for each $\lambda \in m(\Intgr/n)$. We
    know that $u$ can be uniquely written as
    \begin{equation*}
        u = b_0+b_1\sqrt[n]{a}+\cdots+b_{n-1}\sqrt[n]{a}^{n-1}.
    \end{equation*}
    for $b_i\in k$. Then if $\sigma_\lambda(u) = u$, we have
    \begin{align*}
        b_0+ b_1\sqrt[n]{a}\zeta_n^\lambda+\cdots+b_{n-1}\sqrt[n]{a}^{n-1}\zeta_n^{\lambda(n-1)} = b_0+b_1\sqrt[n]{a}+\cdots+b_{n-1}\sqrt[n]{a}^{n-1}.
    \end{align*}
    Hence by the uniqueness of this representation, we have $b_i = \zeta_n^{\lambda i}b_i$ for all $i = 0,\ldots,n-1$,
    and for all $\lambda \in m(\Intgr/n)$. This means that $b_i \neq 0$ if and only if $\lambda i = 0$ in $\Intgr/n$.
    
    That is, there are integers $p$ and $q$ such that $mpi = qn$, so 
    
\end{proof}
        

\end{document}